1.
    
    a:  
    
        ---------- (Axiom)      ---------- (Axiom)
            A                       V
            
            A                       A
        ---------               ----------
          A & A                     V
          
            V                       V
        ---------               ---------
            a                       b
        
            
           
    b:
        
        Consider a&a. This can be gotten from first choosing A&A, then changing the second A to V to get A & V,
        then evaluating V to a, then evaluating the first A to V giving V & a, and evaluating that to a, giving a & a.
        However, this could've been done differently. Instead, we could've done A&A -> V&A -> a&A -> a&V -> a&a.
        
        
        
    c: 
    
        (a^n)(b^m)(c^p), where n >= 1, m >= 0, p >= 1.
        
        
        
    d:
    
        (b^n)(a^m)b, where n >= 1, m >= 2
        
        1.  baab is in the grammer. b = b^1 which is legal, aa = a^2 which is legal, and it ends in a b as required.
        2.  bbab is not in the grammar. There must be two a's at minimum after some positive number of b's, but there
            is only one a.
        3.  bbaaaaa is not in the grammar. The sequence must end with b, and it does not.
        4. bbaab is in the grammar. bb = b^2 which is legal, aa = a^2 which is legal, and it ends in b as required.
        
        
     e: 
     
        1. S -> a, S -> S -> b, S -> c, S -> B -> d. Thus, abcd is valid.
        2. not generated by the grammar.
        3. not generated by the grammar.
        4. not generated by the grammar.
        5. S -> a, S -> S -> c, S -> c, S -> B -> A -> c. Thus, accc is valid.


2. 

    a:   
        i.  First Grammar: Just an operand or a left-associative formula of operands and operators.
            Second Grammar: Just an operand or a right-associative formula of operands and operators.
        ii. The same expressions are generated. With a lack of parantheses, the associativity of the operations
            is not preserved.
            
    b:
        (2 - 1 << 3) + (2 << 3 - 1)
        If - has higher precedence, then we will get [(2-1) << 3] + [2 << (3-1)] = 8 + 8 = 16.
        If << has higher precedence, then we will get [2 - (1 << 3)] + [(2 << 3) - 1] = -6 + 15 = 9.
        This expression returns 16 in Scala, so - has higher precedence than <<.
        
    c:
        S ::= T | 0
        T ::= -P | P | -P.HEP | P.HEP | -P.HE-P | P.HE-P
        P ::= GP | GH
        G ::= 1 | 2 | ... | 9
        H ::= NH | N
        N ::= 0 | 1 | ... | 9
        
        
        
        
           
        